POC: try to compute gmaps via pmap.
This was suggested by Robbert Krebbers, and improves things by a
log, but we're still way too far off (see numbers in the test).

theories/prelude/gmap.v
@@ -5,6 +5,7 @@
  *)
 
 From stdpp Require Export gmap mapset.
+From stdpp Require Import pmap.
 From bedrock.prelude Require Import base fin_sets.
 
 (* To upstream to Iris: using [mapseq_eq] directly would unfold a TC opaque
@@ -50,3 +51,67 @@ Section gset_bind.
     gset_bind f {[ a ]} = f a.
   Proof. set_solver. Qed.
 End gset_bind.
+
+(* Tactic for more efficiently computing a gmap (suggested by Robbert Krebbers). *)
+Module compute_gmap.
+  Definition to_pmap {K V : Type} `{Countable K} : gmap K V -> Pmap V :=
+    map_fold (fun k v pm => <[encode k := v]> pm) ∅.
+
+  Definition of_pmap {K V : Type} `{Countable K} : Pmap V -> gmap K V :=
+    map_fold (fun k v m =>
+      match decode k with
+      | None => m
+      | Some k => <[k := v]> m
+      end) ∅.
+
+  Lemma insert_to_pmap_lookup_Some_decode {K V : Type} `{Countable K}
+      (k : K) (v : V) (m : gmap K V) (j : positive) (w : V) :
+    <[encode k:=v]> (to_pmap m) !! j = Some w → ∃ k, @encode K _ _ k = j.
+  Proof.
+    move => /lookup_insert_Some [].
+    { move => [??]. simplify_eq.  by eexists. }
+    move => [_]. clear. rewrite /to_pmap.
+    elim m using map_ind; clear; first done.
+    move => k v m Hk IH.
+    rewrite map_fold_insert //.
+    - move => /lookup_insert_Some [][??]; [by eexists|by apply IH].
+    - move => ????? Hne *. apply insert_commute => ?. simplify_eq.
+  Qed.
+
+  Lemma to_of_pmap {K V : Type} `{Countable K} :
+    forall (m : gmap K V), of_pmap (to_pmap m) = m.
+  Proof.
+    move => m. rewrite /of_pmap/to_pmap.
+    elim m using map_ind; clear m; first done.
+    move => k v m Hk IH. rewrite -{2}IH{IH}.
+    rewrite !map_fold_insert; [by rewrite decode_encode|..|done].
+    - move => j1 j2 ??? Hne H1 H2.
+      apply insert_to_pmap_lookup_Some_decode in H1 as [k1 H1].
+      apply insert_to_pmap_lookup_Some_decode in H2 as [k2 H2].
+      repeat case_match => //.
+      rewrite insert_commute // => ?. simplify_eq.
+      rewrite ->decode_encode in *. simplify_eq.
+    - revert Hk. elim m using map_ind; first done.
+      move => ???? IH /lookup_insert_None [??].
+      rewrite map_fold_insert => //; intros.
+      + rewrite lookup_insert_ne //. apply IH => //.
+        move => Habs. by apply encode_inj in Habs.
+      + rewrite insert_commute; first done.
+        move => Habs. by apply encode_inj in Habs.
+    - move => *. rewrite insert_commute; first done.
+      move => Habs. by apply encode_inj in Habs.
+  Qed.
+
+  Ltac compute_gmap t :=
+    let ty := type of t in
+    let ty := eval hnf in ty in
+    lazymatch ty with
+    | gmap ?K ?V =>
+        let t := eval vm_compute in (@to_pmap K V _ _ t) in
+        let t :=
+          eval lazy [
+            of_pmap map_fold Pmap_fold pmap.Pmap_fold_aux pmap.Pmap_ne_fold
+          ] in (@of_pmap K V _ _ t)
+        in t
+    end.
+End compute_gmap.
