tests/compute_gmap.t/test.v
@@ -1,0 +1,91 @@
+Require Import bedrock.prelude.gmap.
+Require Import bedrock.lang.cpp.parser.
+
+#[local] Open Scope bs_scope.
+
+Ltac compute_translation_unit t :=
+  let t := eval hnf in t in
+  let symbols := compute_gmap.compute_gmap (t.(symbols)) in
+  let types := compute_gmap.compute_gmap (t.(types)) in
+  let initializer := eval vm_compute in (t.(initializer)) in
+  let byte_order := eval vm_compute in (t.(byte_order)) in
+  exact {| symbols := symbols; types := types; initializer := initializer; byte_order := byte_order |}.
+
+(* 1.7 seconds for 1000 functions, versus 0.8 on master pre-8.18-bump. *)
+(* 38 seconds for 5000 functions, versus 3.5 on master pre-8.18-bump. *)
+(* Way too long for 10000 functions, versus stack overflow on master pre-8.18-bump. *)
+
+Definition module_10 : translation_unit := ltac:(compute_translation_unit constr:(
+  decls (
+    (Dfunction "_Z2f1i"
+      (Build_Func Tint
+        (("x", Tint) :: nil) CC_C Ar_Definite
+        (Some (Impl
+            (Sseq (
+                (Sreturn_val
+                  (Ecast Cl2r (Evar (Lname "x") Tint) Prvalue Tint)) :: nil)))))) ::
+    (Dfunction "_Z2f2i"
+      (Build_Func Tint
+        (("x", Tint) :: nil) CC_C Ar_Definite
+        (Some (Impl
+            (Sseq (
+                (Sreturn_val
+                  (Ecast Cl2r (Evar (Lname "x") Tint) Prvalue Tint)) :: nil)))))) ::
+    (Dfunction "_Z2f3i"
+      (Build_Func Tint
+        (("x", Tint) :: nil) CC_C Ar_Definite
+        (Some (Impl
+            (Sseq (
+                (Sreturn_val
+                  (Ecast Cl2r (Evar (Lname "x") Tint) Prvalue Tint)) :: nil)))))) ::
+    (Dfunction "_Z2f4i"
+      (Build_Func Tint
+        (("x", Tint) :: nil) CC_C Ar_Definite
+        (Some (Impl
+            (Sseq (
+                (Sreturn_val
+                  (Ecast Cl2r (Evar (Lname "x") Tint) Prvalue Tint)) :: nil)))))) ::
+    (Dfunction "_Z2f5i"
+      (Build_Func Tint
+        (("x", Tint) :: nil) CC_C Ar_Definite
+        (Some (Impl
+            (Sseq (
+                (Sreturn_val
+                  (Ecast Cl2r (Evar (Lname "x") Tint) Prvalue Tint)) :: nil)))))) ::
+    (Dfunction "_Z2f6i"
+      (Build_Func Tint
+        (("x", Tint) :: nil) CC_C Ar_Definite
+        (Some (Impl
+            (Sseq (
+                (Sreturn_val
+                  (Ecast Cl2r (Evar (Lname "x") Tint) Prvalue Tint)) :: nil)))))) ::
+    (Dfunction "_Z2f7i"
+      (Build_Func Tint
+        (("x", Tint) :: nil) CC_C Ar_Definite
+        (Some (Impl
+            (Sseq (
+                (Sreturn_val
+                  (Ecast Cl2r (Evar (Lname "x") Tint) Prvalue Tint)) :: nil)))))) ::
+    (Dfunction "_Z2f8i"
+      (Build_Func Tint
+        (("x", Tint) :: nil) CC_C Ar_Definite
+        (Some (Impl
+            (Sseq (
+                (Sreturn_val
+                  (Ecast Cl2r (Evar (Lname "x") Tint) Prvalue Tint)) :: nil)))))) ::
+    (Dfunction "_Z2f9i"
+      (Build_Func Tint
+        (("x", Tint) :: nil) CC_C Ar_Definite
+        (Some (Impl
+            (Sseq (
+                (Sreturn_val
+                  (Ecast Cl2r (Evar (Lname "x") Tint) Prvalue Tint)) :: nil)))))) ::
+    (Dfunction "_Z3f10i"
+      (Build_Func Tint
+        (("x", Tint) :: nil) CC_C Ar_Definite
+        (Some (Impl
+            (Sseq (
+                (Sreturn_val
+                  (Ecast Cl2r (Evar (Lname "x") Tint) Prvalue Tint)) :: nil)))))) ::
+    nil
+  ) Little)).
